Note problem with env to texec theorem statement

PFun.v
@@ -5,6 +5,9 @@ Require Import FunctionalExtensionality.
 Definition EqDec A := forall (x y:A), {x=y}+{x<>y}.
 Existing Class EqDec.
 
+Definition eq_dec {A} {dec:EqDec A} x y : {x=y}+{x<>y}
+  := dec x y.
+
 Definition pfun A V := A -> option V.
 
 Definition upd A {AEQ: EqDec A} V (m: pfun A V) a v : pfun A V :=
@@ -38,6 +41,25 @@ Qed.
 Hint Rewrite upd_eq  : upd.
 Hint Rewrite upd_neq using (solve [ auto ]) : upd.
 
+Theorem upd_commute : forall A {AEQ:EqDec A} V (m: pfun A V) a v a' v',
+    a <> a' ->
+    upd (upd m a v) a' v' = upd (upd m a' v') a v.
+Proof.
+  unfold upd; intros.
+  extensionality a''.
+  repeat destruct_match.
+Qed.
+
+Theorem upd_repeat : forall A {AEQ:EqDec A} V (m: pfun A V) a v v',
+    upd (upd m a v) a v' = upd m a v'.
+Proof.
+  unfold upd; intros.
+  extensionality a''.
+  destruct_match.
+Qed.
+
+Hint Rewrite upd_repeat : upd.
+
 Definition remove A {AEQ: EqDec A} V (m: pfun A V) a : pfun A V :=
   fun a' => if AEQ a a' then None else m a'.
 
@@ -66,4 +88,31 @@ Proof.
   intros.
   extensionality a'.
   destruct (AEQ a a'); subst; autorewrite with upd; auto.
+Qed.
+
+Theorem remove_none : forall A {AEQ:EqDec A} V (m: pfun A V) a,
+    m a = None ->
+    remove m a = m.
+Proof.
+  unfold remove; intros.
+  extensionality a'.
+  destruct_match.
+Qed.
+
+Theorem upd_remove : forall A {AEQ:EqDec A} V (m: pfun A V) a v,
+    remove (upd m a v) a = remove m a.
+Proof.
+  unfold remove; intros; extensionality a'.
+  destruct_match; autorewrite with upd; auto.
+Qed.
+
+Hint Rewrite upd_remove : upd.
+Hint Rewrite remove_none using (solve [ auto ]) : upd.
+
+Theorem upd_remove_commute : forall A {AEQ:EqDec A} V (m: pfun A V) a v a',
+    a <> a' ->
+    upd (remove m a) a' v = remove (upd m a' v) a.
+Proof.
+  unfold upd, remove; intros; extensionality a''.
+  repeat destruct_match.
 Qed.
